steps

example_chat.thy
@@ -42,14 +42,59 @@ definition lsInit :: "localState" where
 \<rparr>"
 
 
+definition "message_author_assign \<equiv> ''message_author_assign''"
+definition "message_content_assign \<equiv> ''message_content_assign''"
+definition "message_chat_assign \<equiv> ''message_chat_assign''"
+definition "chat_add \<equiv> ''chat_add''"
+definition "message_exists \<equiv> ''message_exists''"
+definition "chat_remove \<equiv> ''chat_remove''"
+definition "message_delete \<equiv> ''message_delete''"
+definition "message_chat_read \<equiv> ''message_chat_read''"
+definition "message_content_read \<equiv> ''message_content_read''"
+definition "message_author_read \<equiv> ''message_author_read''"
+definition "sendMessage \<equiv> ''sendMessage''"
+definition "editMessage \<equiv> ''editMessage''"
+definition "deleteMessage \<equiv> ''deleteMessage''"
+definition "chat_contains \<equiv> ''chat_contains''"
+
+lemma constants_distinct:
+"distinct [message_author_assign, message_content_assign, message_chat_assign, chat_add, message_exists, chat_remove, message_delete, message_chat_read, 
+  sendMessage, editMessage, deleteMessage, message_content_read, message_author_read, chat_contains]"
+  by (auto simp add: message_author_assign_def message_content_assign_def message_chat_assign_def chat_add_def message_exists_def chat_remove_def message_delete_def message_chat_read_def
+sendMessage_def editMessage_def deleteMessage_def message_author_read_def message_content_read_def chat_contains_def)
+
+
+
+lemma distinct_unfold1: "distinct [] \<longleftrightarrow> True"
+  by auto
+
+lemma distinct_unfold2: "distinct (x#xs) \<longleftrightarrow> x \<notin> set xs \<and> distinct xs"
+  by auto
+
+lemma distinct_unfold3: "a\<notin>set(x#xs) \<longleftrightarrow> a \<noteq> x \<and> x \<noteq> a \<and> a\<notin>set xs"
+  by auto
+
+lemma distinct_unfold4: "a\<notin>set[] \<longleftrightarrow> True"
+  by auto
+
+find_theorems "_ \<and> _ \<and> _"
+
+schematic_goal constants_distinct2[simp]: "?P"
+  apply (insert constants_distinct)
+  apply (subst(asm) distinct_unfold1 distinct_unfold2 distinct_unfold3 distinct_unfold4 simp_thms(21) conj_assoc)+
+  apply assumption
+  done
+
+
+
 definition sendMessageImpl :: "(localState, val) procedureImpl" where
   "sendMessageImpl ls \<equiv> [
    (* 0 *) BeginAtomic (ls\<lparr>ls_pc := 1\<rparr>),
    (* 1 *) NewId (\<lambda>x. (ls\<lparr>ls_t := x, ls_pc := 2\<rparr> :: localState)),
-   (* 2 *) DbOperation ''message_author_assign'' [ls_t ls, ls_from ls] (\<lambda>r. ls\<lparr>ls_pc := 3\<rparr>),
-   (* 3 *) DbOperation ''message_content_assign'' [ls_t ls, ls_content ls] (\<lambda>r. ls\<lparr>ls_pc := 4\<rparr>),
-   (* 4 *) DbOperation ''message_chat_assign'' [ls_t ls, ls_from ls] (\<lambda>r. ls\<lparr>ls_pc := 5\<rparr>),
-   (* 5 *) DbOperation ''chat_add'' [ls_to ls, ls_t ls] (\<lambda>r. ls\<lparr>ls_pc := 6\<rparr>),
+   (* 2 *) DbOperation message_author_assign [ls_t ls, ls_from ls] (\<lambda>r. ls\<lparr>ls_pc := 3\<rparr>),
+   (* 3 *) DbOperation message_content_assign [ls_t ls, ls_content ls] (\<lambda>r. ls\<lparr>ls_pc := 4\<rparr>),
+   (* 4 *) DbOperation message_chat_assign [ls_t ls, ls_from ls] (\<lambda>r. ls\<lparr>ls_pc := 5\<rparr>),
+   (* 5 *) DbOperation chat_add [ls_to ls, ls_t ls] (\<lambda>r. ls\<lparr>ls_pc := 6\<rparr>),
    (* 6 *) EndAtomic (ls\<lparr>ls_pc := 6\<rparr>),
    (* 7 *) Return (ls_t ls)
    ] ! ls_pc ls"
@@ -57,8 +102,8 @@ definition sendMessageImpl :: "(localState, val) procedureImpl" where
 definition editMessageImpl :: "(localState, val) procedureImpl" where
   "editMessageImpl ls \<equiv> [
    (* 0 *) BeginAtomic (ls\<lparr>ls_pc := 1\<rparr>),
-   (* 1 *) DbOperation ''message_exists'' [ls_id ls] (\<lambda>r. if r = Bool True then ls\<lparr>ls_pc := 2\<rparr> else ls\<lparr>ls_pc := 3\<rparr>),
-   (* 2 *) DbOperation ''message_content_assign'' [ls_id ls, ls_content ls] (\<lambda>r. ls\<lparr>ls_pc := 3\<rparr>),
+   (* 1 *) DbOperation message_exists [ls_id ls] (\<lambda>r. if r = Bool True then ls\<lparr>ls_pc := 2\<rparr> else ls\<lparr>ls_pc := 3\<rparr>),
+   (* 2 *) DbOperation message_content_assign [ls_id ls, ls_content ls] (\<lambda>r. ls\<lparr>ls_pc := 3\<rparr>),
    (* 3 *) EndAtomic  (ls\<lparr>ls_pc := 4\<rparr>),
    (* 4 *) Return Undef
    ] ! ls_pc ls"   
@@ -66,9 +111,9 @@ definition editMessageImpl :: "(localState, val) procedureImpl" where
 definition deleteMessageImpl :: "(localState, val) procedureImpl" where
   "deleteMessageImpl ls \<equiv> [
    (* 0 *) BeginAtomic (ls\<lparr>ls_pc := 1\<rparr>),
-   (* 1 *) DbOperation ''message_chat_read'' [ls_id ls] (\<lambda>r. ls\<lparr>ls_pc := 2, ls_c := r\<rparr>),
-   (* 2 *) DbOperation ''chat_remove'' [ls_c ls, ls_id ls] (\<lambda>r. ls\<lparr>ls_pc := 3\<rparr>),
-   (* 3 *) DbOperation ''message_delete'' [ls_id ls] (\<lambda>r. ls\<lparr>ls_pc := 4\<rparr>),
+   (* 1 *) DbOperation message_chat_read [ls_id ls] (\<lambda>r. ls\<lparr>ls_pc := 2, ls_c := r\<rparr>),
+   (* 2 *) DbOperation chat_remove [ls_c ls, ls_id ls] (\<lambda>r. ls\<lparr>ls_pc := 3\<rparr>),
+   (* 3 *) DbOperation message_delete [ls_id ls] (\<lambda>r. ls\<lparr>ls_pc := 4\<rparr>),
    (* 4 *) EndAtomic  (ls\<lparr>ls_pc := 5\<rparr>),
    (* 5 *) Return Undef
    ] ! ls_pc ls"      
@@ -76,17 +121,17 @@ definition deleteMessageImpl :: "(localState, val) procedureImpl" where
 
 definition procedures where
   "procedures proc args \<equiv> 
-  if proc = ''sendMessage'' then
+  if proc = sendMessage then
     case args of 
       [UserId from, String content, ChatId to] \<Rightarrow> 
         Some (lsInit\<lparr>ls_from := UserId from, ls_content := String content, ls_to := ChatId to \<rparr> , sendMessageImpl)
       | _ \<Rightarrow> None
-  else if proc = ''editMessage'' then 
+  else if proc = editMessage then 
     case args of 
       [MessageId i] \<Rightarrow> 
         Some (lsInit\<lparr>ls_id := MessageId i \<rparr> , editMessageImpl)
       | _ \<Rightarrow> None
-  else if proc = ''deleteMessage'' then 
+  else if proc = deleteMessage then 
     case args of 
       [MessageId i] \<Rightarrow> 
         Some (lsInit\<lparr>ls_id := MessageId i \<rparr> , deleteMessageImpl)
@@ -102,55 +147,56 @@ definition "callsWithOpArgsH ctxt_calls opName args \<equiv> {c. ctxt_calls c \<
 
 abbreviation "callsWithOpArgs ctxt opName args \<equiv> callsWithOpArgsH (calls ctxt) opName args"
 
-
+(*
 definition latest_name_assign :: "val operationContext \<Rightarrow> val \<Rightarrow> val set" where
   "latest_name_assign ctxt u \<equiv>  {v | c1 v. 
-     (c1, [u, v]) \<in> callsOfOp ctxt ''users_name_assign''
-   \<and> (\<forall>c2\<in>callsWithOpArgs ctxt ''users_remove'' [u]. (c2,c1)\<in>happensBefore ctxt)
-   \<and> (\<forall>(c2, args) \<in> callsOfOp ctxt ''users_name_assign''. args!0 = u \<longrightarrow> \<not>(c1,c2)\<in>happensBefore ctxt)}"
+     (c1, [u, v]) \<in> callsOfOp ctxt users_name_assign
+   \<and> (\<forall>c2\<in>callsWithOpArgs ctxt users_remove [u]. (c2,c1)\<in>happensBefore ctxt)
+   \<and> (\<forall>(c2, args) \<in> callsOfOp ctxt users_name_assign. args!0 = u \<longrightarrow> \<not>(c1,c2)\<in>happensBefore ctxt)}"
 
 definition latest_mail_assign :: "val operationContext \<Rightarrow> val \<Rightarrow> val set" where
   "latest_mail_assign ctxt u \<equiv>  {v | c1 v. 
-     (c1, [u, v]) \<in> callsOfOp ctxt ''users_mail_assign''
-   \<and> (\<forall>c2\<in>callsWithOpArgs ctxt ''users_remove'' [u]. (c2,c1)\<in>happensBefore ctxt)
-   \<and> (\<forall>(c2, args) \<in> callsOfOp ctxt ''users_mail_assign''. args!0 = u \<longrightarrow> \<not>(c1,c2)\<in>happensBefore ctxt)}"   
+     (c1, [u, v]) \<in> callsOfOp ctxt users_mail_assign
+   \<and> (\<forall>c2\<in>callsWithOpArgs ctxt users_remove [u]. (c2,c1)\<in>happensBefore ctxt)
+   \<and> (\<forall>(c2, args) \<in> callsOfOp ctxt users_mail_assign. args!0 = u \<longrightarrow> \<not>(c1,c2)\<in>happensBefore ctxt)}"   
+*)
 
 definition crdtSpec_message_chat_read :: "val list \<Rightarrow> val operationContext \<Rightarrow> val \<Rightarrow> bool" where
   "crdtSpec_message_chat_read args ctxt res \<equiv> \<exists>l.
   res = ListVal l 
  \<and> (\<forall>v. v\<in>set l \<longleftrightarrow> 
-   (\<exists>c1\<in>callsWithOpArgs ctxt ''message_chat_assign'' (args@[v]).
-       (\<forall>(c2,args')\<in>callsOfOp ctxt ''message_chat_assign''. take 1 args' = args \<longrightarrow> (c1,c2)\<notin>happensBefore ctxt)
-     \<and> (\<forall>c2\<in>callsWithOpArgs ctxt ''message_delete'' args. (c2,c1)\<in>happensBefore ctxt)))"
+   (\<exists>c1\<in>callsWithOpArgs ctxt message_chat_assign (args@[v]).
+       (\<forall>(c2,args')\<in>callsOfOp ctxt message_chat_assign. (\<exists>chat. args' = args@[chat]) \<longrightarrow> (c1,c2)\<notin>happensBefore ctxt)
+     \<and> (\<forall>c2\<in>callsWithOpArgs ctxt message_delete args. (c2,c1)\<in>happensBefore ctxt)))"
 
 definition crdtSpec_message_author_read :: "val list \<Rightarrow> val operationContext \<Rightarrow> val \<Rightarrow> bool" where
   "crdtSpec_message_author_read args ctxt res \<equiv> \<exists>l.
   res = ListVal l 
  \<and> (\<forall>v. v\<in>set l \<longleftrightarrow> 
-    (\<exists>c1\<in>callsWithOpArgs ctxt ''message_author_assign'' (args@[v]).
-       (\<forall>(c2,args')\<in>callsOfOp ctxt ''message_author_assign''. take 1 args' = args \<longrightarrow> (c1,c2)\<notin>happensBefore ctxt)
-     \<and> (\<forall>c2\<in>callsWithOpArgs ctxt ''message_delete'' args. (c2,c1)\<in>happensBefore ctxt)))"
+    (\<exists>c1\<in>callsWithOpArgs ctxt message_author_assign (args@[v]).
+       (\<forall>(c2,args')\<in>callsOfOp ctxt message_author_assign. (\<exists>author. args' = args@[author]) \<longrightarrow> (c1,c2)\<notin>happensBefore ctxt)
+     \<and> (\<forall>c2\<in>callsWithOpArgs ctxt message_delete args. (c2,c1)\<in>happensBefore ctxt)))"
 
 definition is_message_updateH  where
   (*:: "val operationContext \<Rightarrow> callId \<Rightarrow> val \<Rightarrow> bool" where *)
   "is_message_updateH mid c \<equiv> 
   case c of 
-     Call upd (mid'#args) _ \<Rightarrow> upd \<in> {''message_author_assign'', ''message_content_assign'', ''message_chat_assign''} \<and> mid = mid' 
+     Call upd (mid'#args) _ \<Rightarrow> upd \<in> {message_author_assign, message_content_assign, message_chat_assign} \<and> mid = mid' 
    | _ \<Rightarrow> False"
 
-lemma is_message_updateH_simp: "is_message_updateH mid (Call upd (mid'#args) res) \<longleftrightarrow> upd \<in> {''message_author_assign'', ''message_content_assign'', ''message_chat_assign''} \<and> mid = mid'"
+lemma is_message_updateH_simp: "is_message_updateH mid (Call upd (mid'#args) res) \<longleftrightarrow> upd \<in> {message_author_assign, message_content_assign, message_chat_assign} \<and> mid = mid'"
   by (auto simp add: is_message_updateH_def)
 
-lemma is_message_updateH_simp1[simp]: "is_message_updateH mid (Call ''message_author_assign'' (mid'#args) res) \<longleftrightarrow> mid = mid'"
+lemma is_message_updateH_simp1[simp]: "is_message_updateH mid (Call message_author_assign (mid'#args) res) \<longleftrightarrow> mid = mid'"
   by (auto simp add: is_message_updateH_def)
 
-lemma is_message_updateH_simp2[simp]: "is_message_updateH mid (Call ''message_content_assign'' (mid'#args) res) \<longleftrightarrow> mid = mid'"
+lemma is_message_updateH_simp2[simp]: "is_message_updateH mid (Call message_content_assign (mid'#args) res) \<longleftrightarrow> mid = mid'"
   by (auto simp add: is_message_updateH_def)
 
-lemma is_message_updateH_simp3[simp]: "is_message_updateH mid (Call ''message_chat_assign'' (mid'#args) res) \<longleftrightarrow> mid = mid'"
+lemma is_message_updateH_simp3[simp]: "is_message_updateH mid (Call message_chat_assign (mid'#args) res) \<longleftrightarrow> mid = mid'"
   by (auto simp add: is_message_updateH_def)
 
-lemma is_message_updateH_simp4[simp]: "  \<not>is_message_updateH mid (Call upd (mid'#args) res)" if "upd \<notin> {''message_author_assign'', ''message_content_assign'', ''message_chat_assign''}"
+lemma is_message_updateH_simp4[simp]: "  \<not>is_message_updateH mid (Call upd (mid'#args) res)" if "upd \<notin> {message_author_assign, message_content_assign, message_chat_assign}"
   using that  by (auto simp add: is_message_updateH_def )
 
 definition message_updates :: "(callId \<rightharpoonup> val call) \<Rightarrow> val \<Rightarrow> callId set" where
@@ -166,12 +212,12 @@ definition crdtSpec_message_exists_h :: "val list \<Rightarrow> val operationCon
   \<exists>mId.
   args = [mId]
  \<and> (\<exists>c. is_message_update ctxt c mId)
- \<and> (\<forall>c\<in>callsWithOpArgs ctxt ''message_delete'' args. 
+ \<and> (\<forall>c\<in>callsWithOpArgs ctxt message_delete args. 
           (\<exists>c'. (c,c')\<in>happensBefore ctxt \<and> is_message_update ctxt c mId))"
 
 schematic_goal crdtSpec_message_exists_h_def2:
 "crdtSpec_message_exists_h [mId] ctxt = ((\<exists>c. is_message_update ctxt c mId)
- \<and> (\<forall>c\<in>callsWithOpArgs ctxt ''message_delete'' [mId]. 
+ \<and> (\<forall>c\<in>callsWithOpArgs ctxt message_delete [mId]. 
           (\<exists>c'. (c,c')\<in>happensBefore ctxt \<and> is_message_update ctxt c mId)))"
   by (auto simp add: crdtSpec_message_exists_h_def)
 
@@ -182,8 +228,8 @@ definition crdtSpec_message_exists :: "val list \<Rightarrow> val operationConte
 (* ignores map-deletes as they are not used *)
 definition crdtSpec_chat_contains_h :: "val list \<Rightarrow> val operationContext \<Rightarrow> bool" where
   "crdtSpec_chat_contains_h args ctxt \<equiv> 
-  (callsWithOpArgs ctxt ''chat_add'' args \<noteq> {})
-  \<and> (\<forall>cr\<in>callsWithOpArgs  ctxt ''chat_remove'' args. (\<exists>ca\<in>callsWithOpArgs ctxt ''chat_add'' args. (cr,ca) \<in> happensBefore ctxt))"
+  (callsWithOpArgs ctxt chat_add args \<noteq> {})
+  \<and> (\<forall>cr\<in>callsWithOpArgs  ctxt chat_remove args. (\<exists>ca\<in>callsWithOpArgs ctxt chat_add args. (cr,ca) \<in> happensBefore ctxt))"
 
 definition crdtSpec_chat_contains :: "val list \<Rightarrow> val operationContext \<Rightarrow> val \<Rightarrow> bool" where
   "crdtSpec_chat_contains args ctxt res \<equiv> 
@@ -192,10 +238,10 @@ definition crdtSpec_chat_contains :: "val list \<Rightarrow> val operationContex
 
 definition crdtSpec :: "operation \<Rightarrow> val list \<Rightarrow> val operationContext \<Rightarrow> val \<Rightarrow> bool" where
   "crdtSpec oper  \<equiv> 
-  if oper = ''message_chat_read'' then crdtSpec_message_chat_read
-  else if oper = ''message_author_read'' then crdtSpec_message_author_read
-  else if oper = ''chat_contains'' then crdtSpec_chat_contains
-  else if oper = ''message_exists'' then crdtSpec_message_exists
+  if oper = message_chat_read then crdtSpec_message_chat_read
+  else if oper = message_author_read then crdtSpec_message_author_read
+  else if oper = chat_contains then crdtSpec_chat_contains
+  else if oper = message_exists then crdtSpec_message_exists
   else 
     (* other operations are updates and don't have a result *)
     (\<lambda>args ctxt res. res = Undef)"
@@ -241,16 +287,24 @@ lemma mkContext_happensBefore_contains_simps: "(c1,c2) \<in> happensBefore (mkCo
 
 lemmas mkContext_simps = mkContext_happensBefore_contains_simps mkContext_calls_eq_simps
 
-(* property 1 *)
+(* property 1:
+If the chat contains a reference to a message, the message exists
+ *)
 definition inv1 :: "val invariantContext \<Rightarrow> bool" where
   "inv1 ctxt \<equiv> \<forall>c m. crdtSpec_chat_contains_h [c,m] (mkContext ctxt) \<longrightarrow> crdtSpec_message_exists_h [m] (mkContext ctxt)"
 
-(* property 2 *)
+(* property 2:
+If a message exists, there is exactly one author set for the message 
+We know this, because we never update the author...
+*)
 definition inv2 :: "val invariantContext \<Rightarrow> bool" where
   "inv2 ctxt \<equiv> \<forall>m. crdtSpec_message_exists_h [m] (mkContext ctxt) \<longrightarrow> (\<exists>a. crdtSpec_message_author_read [m] (mkContext ctxt) (ListVal [a]))"
 
+(*
+There are no updates to a message after it has been deleted
+*)
 definition inv2_h1 :: "val invariantContext \<Rightarrow> bool" where
-  "inv2_h1 ctxt \<equiv> (\<forall>c mId. calls ctxt c \<triangleq> Call ''message_delete'' [mId] Undef \<longrightarrow> (\<nexists>c'. is_message_update ctxt c' mId \<and> (c,c')\<in>happensBefore ctxt ))"
+  "inv2_h1 ctxt \<equiv> (\<forall>c mId. calls ctxt c \<triangleq> Call message_delete [mId] Undef \<longrightarrow> (\<nexists>c'. is_message_update ctxt c' mId \<and> (c,c')\<in>happensBefore ctxt ))"
 
 
 definition inv :: "val invariantContext \<Rightarrow> bool" where
@@ -477,13 +531,13 @@ qed
 
 lemma every_query_has_result_message_chat_read:
   assumes "finite (dom (calls ctxt))"
-  shows  "\<exists>res. crdtSpec ''message_chat_read'' args ctxt res"
+  shows  "\<exists>res. crdtSpec message_chat_read args ctxt res"
   apply (auto simp add: crdtSpec_def)
   apply (rule Ex_quantor)
   apply (auto simp add: crdtSpec_message_chat_read_def )
   apply (rule finite_list_exists)
 
-  apply (rule_tac B="{v. \<exists>c. calls ctxt c \<triangleq> Call ''message_chat_assign'' (args @ [v]) Undef}" in finite_subset)
+  apply (rule_tac B="{v. \<exists>c. calls ctxt c \<triangleq> Call message_chat_assign (args @ [v]) Undef}" in finite_subset)
    apply (auto simp add: callsWithOpArgsH_def)
   apply (rule finite_mapping3[OF `finite (dom (calls ctxt))`])
   by (meson append1_eq_conv call.inject injI)
@@ -491,50 +545,53 @@ lemma every_query_has_result_message_chat_read:
 
 lemma every_query_has_result_message_author_read:
   assumes "finite (dom (calls ctxt))"
-  shows  "\<exists>res. crdtSpec ''message_author_read'' args ctxt res"
+  shows  "\<exists>res. crdtSpec message_author_read args ctxt res"
   apply (auto simp add: crdtSpec_def)
   apply (rule Ex_quantor)
   apply (auto simp add: crdtSpec_message_author_read_def)
   apply (rule finite_list_exists)
-  apply (rule_tac B="{v. \<exists>c. calls ctxt c \<triangleq> Call ''message_author_assign'' (args @ [v]) Undef}" in finite_subset)
+  apply (rule_tac B="{v. \<exists>c. calls ctxt c \<triangleq> Call message_author_assign (args @ [v]) Undef}" in finite_subset)
    apply (auto simp add: callsWithOpArgsH_def)
   apply (rule finite_mapping3[OF `finite (dom (calls ctxt))`])
   by (meson append1_eq_conv call.inject injI)
 
 lemma every_query_has_result_chat_contains[simp]:
-  shows  "\<exists>res. crdtSpec ''chat_contains'' args ctxt res"
+  shows  "\<exists>res. crdtSpec chat_contains args ctxt res"
   apply (auto simp add: crdtSpec_def)
   by (auto simp add: crdtSpec_chat_contains_def)
 
 lemma every_query_has_result_message_exists[simp]:
-  shows  "\<exists>res. crdtSpec ''message_exists'' args ctxt res"
+  shows  "\<exists>res. crdtSpec message_exists args ctxt res"
   apply (auto simp add: crdtSpec_def)
   by (auto simp add: crdtSpec_message_exists_def)
 
 lemma every_query_has_result_assign[simp]:
-  shows "crdtSpec ''message_author_assign'' args ctxt res \<longleftrightarrow> res = Undef"
-"crdtSpec ''message_content_assign'' args ctxt res \<longleftrightarrow> res = Undef"
-"crdtSpec ''message_chat_assign'' args ctxt res \<longleftrightarrow> res = Undef"
-"crdtSpec ''chat_add'' args ctxt res \<longleftrightarrow> res = Undef"
-"crdtSpec ''chat_remove'' args ctxt res \<longleftrightarrow> res = Undef"
-"crdtSpec ''message_delete'' args ctxt res \<longleftrightarrow> res = Undef"
+  shows "crdtSpec message_author_assign args ctxt res \<longleftrightarrow> res = Undef"
+"crdtSpec message_content_assign args ctxt res \<longleftrightarrow> res = Undef"
+"crdtSpec message_chat_assign args ctxt res \<longleftrightarrow> res = Undef"
+"crdtSpec chat_add args ctxt res \<longleftrightarrow> res = Undef"
+"crdtSpec chat_remove args ctxt res \<longleftrightarrow> res = Undef"
+"crdtSpec message_delete args ctxt res \<longleftrightarrow> res = Undef"
   by (auto simp add: crdtSpec_def)
 
 lemma every_query_has_result:
   assumes fin: "finite (dom (calls ctxt))"
   shows  "\<exists>res. crdtSpec procName args ctxt res"
-  apply (case_tac "procName = ''message_chat_read''"; case_tac "procName = ''message_author_read''"; case_tac "procName = ''chat_contains''"; case_tac "procName = ''message_exists''")
+  apply (case_tac "procName = message_chat_read"; case_tac "procName = message_author_read"; case_tac "procName = chat_contains"; case_tac "procName = message_exists")
                  apply (auto simp add: every_query_has_result_message_chat_read[OF fin] every_query_has_result_message_author_read[OF fin])
   apply (auto simp add: crdtSpec_def )
   done
 
 
+
 lemma commitedCalls_simps[simp]:
-  assumes noUncommitted: "\<And>tx. transactionStatus S tx \<noteq> Some Uncommited"
+  assumes noUncommitted: "\<And>tx. tx\<in>Option.these(range (callOrigin S)) \<Longrightarrow>  transactionStatus S tx \<noteq> Some Uncommited"
     and wf: "state_wellFormed S"
   shows "commitedCalls S = dom (calls S)"
   using assms apply (auto simp add: commitedCallsH_def isCommittedH_def domD domIff wellFormed_callOrigin_dom3)
-  by (smt not_Some_eq transactionStatus.exhaust wellFormed_callOrigin_dom3 wf_no_transactionStatus_origin_for_nothing)
+  by (smt domD domIff in_these_eq option.distinct(1) rangeI transactionStatus.exhaust wellFormed_callOrigin_dom wellFormed_state_callOrigin_transactionStatus)
+
+
 
 lemma consistentSnapshot_vis_subset[dest]:
   assumes "consistentSnapshot S vis"
@@ -745,7 +802,14 @@ lemma message_updates_update_simps[simp]:
       = message_updates cs mId \<union> (if is_message_updateH mId (Call opName args res) then {c} else {})"
   using assms  by (auto simp add: message_updates_def)
 
+lemma restrict_map_dom[simp]: "m |` dom m = m" for m
+  by (auto simp add: restrict_map_def domD domIff)
 
+lemma dom_exists: "x\<in>dom m \<longleftrightarrow> (\<exists>y. m x \<triangleq> y)"
+  by auto
+
+lemma exists_eq_simp: "(\<exists>a. \<forall>v. (v=a) \<longleftrightarrow> P a v) \<longleftrightarrow> (\<exists>a. P a a \<and> (\<forall>v. v\<noteq>a \<longrightarrow> \<not>P a v))"
+  by auto
 
 theorem "programCorrect progr"
 proof (rule show_correctness_via_single_session)
@@ -843,7 +907,7 @@ proof (rule show_correctness_via_single_session)
       proof (auto simp add: procedures_def split: if_splits list.splits val.splits)
         text {* Procedure editMessage *}
         fix mId
-        assume a0: "invocationOp S i \<triangleq> (''editMessage'', [MessageId mId])"
+        assume a0: "invocationOp S i \<triangleq> (editMessage, [MessageId mId])"
           and a1[simp]: "currentProc S i \<triangleq> editMessageImpl"
           and a2[simp]: "localState S i \<triangleq> lsInit\<lparr>ls_id := MessageId mId\<rparr>"
           and a3: "uniqueIdsInList [MessageId mId] \<subseteq> knownIds S"
@@ -857,7 +921,7 @@ proof (rule show_correctness_via_single_session)
         show "checkCorrect progr S i"
         proof (auto simp add: checkCorrect_simps editMessageImpl_def updateHb_chain; (subst invariant_all_def)?; auto? )
 
-          show "example_chat.inv (invContextH (callOrigin S'(c \<mapsto> t, ca \<mapsto> t)) (transactionOrigin S') (transactionStatus S'(t \<mapsto> Commited)) (updateHb (happensBefore S') vis [c, ca]) (calls S'(c \<mapsto> Call ''message_exists'' [MessageId mId] (Bool True), ca \<mapsto> Call ''message_content_assign'' [MessageId mId, ls_content lsInit] Undef)) (knownIds S') (invocationOp S') (invocationRes S') (Some visa))"
+          show "example_chat.inv (invContextH (callOrigin S'(c \<mapsto> t, ca \<mapsto> t)) (transactionOrigin S') (transactionStatus S'(t \<mapsto> Commited)) (updateHb (happensBefore S') vis [c, ca]) (calls S'(c \<mapsto> Call message_exists [MessageId mId] (Bool True), ca \<mapsto> Call message_content_assign [MessageId mId, ls_content lsInit] Undef)) (knownIds S') (invocationOp S') (invocationRes S') (Some visa))"
             if c0: "transactionStatus S t = None"
               and c1: "invariant_all S'"
               and c2[simp]: "state_wellFormed S'"
@@ -868,16 +932,39 @@ proof (rule show_correctness_via_single_session)
               and c7: "transactionOrigin S' t \<triangleq> i"
               and c15: "\<forall>c. callOrigin S' c \<noteq> Some t"
               and c8[simp]: "calls S' c = None"
-              and c9: "crdtSpec ''message_exists'' [MessageId mId] (getContextH (calls S') (happensBefore S') (Some vis)) (Bool True)"
+              and c9: "crdtSpec message_exists [MessageId mId] (getContextH (calls S') (happensBefore S') (Some vis)) (Bool True)"
               and c10: "visibleCalls S' i \<triangleq> vis"
               and c11[simp]: "ca \<noteq> c"
               and c12[simp]: "calls S' ca = None"
               and no_uncommitted[simp]: "\<forall>ta. ta \<noteq> t \<longrightarrow> transactionStatus S' ta \<noteq> Some Uncommited"
-              and c14[simp]: "consistentSnapshotH (calls S'(c \<mapsto> Call ''message_exists'' [MessageId mId] (Bool True), ca \<mapsto> Call ''message_content_assign'' [MessageId mId, ls_content lsInit] Undef)) (updateHb (happensBefore S') vis [c, ca]) (callOrigin S'(c \<mapsto> t, ca \<mapsto> t)) (transactionStatus S'(t \<mapsto> Commited)) visa"
+              and c14[simp]: "consistentSnapshotH (calls S'(c \<mapsto> Call message_exists [MessageId mId] (Bool True), ca \<mapsto> Call message_content_assign [MessageId mId, ls_content lsInit] Undef)) (updateHb (happensBefore S') vis [c, ca]) (callOrigin S'(c \<mapsto> t, ca \<mapsto> t)) (transactionStatus S'(t \<mapsto> Commited)) visa"
             for  t S' c vis ca visa
           proof (subst invContextH_simps_allCommitted; simp?)
             have [simp]: "c \<noteq> ca"
-                using c11 by blast
+              using c11 by blast
+
+            from c14 
+            have visa_subset: "visa \<subseteq> dom(calls S') \<union> {c, ca}"
+              by (auto simp add: consistentSnapshotH_def)
+
+            hence visa'_subset: "visa - {c,ca} \<subseteq> dom(calls S')"
+              by auto
+
+            hence visa_calls: "\<And>c1. \<lbrakk>c1 \<in> visa; c1 \<noteq> c; c1 \<noteq> ca\<rbrakk> \<Longrightarrow> calls S' c1 \<noteq> None"
+              by blast
+
+
+            hence visa_callOrigin: "\<And>c1. \<lbrakk>c1 \<in> visa; c1 \<noteq> c; c1 \<noteq> ca\<rbrakk> \<Longrightarrow> callOrigin S' c1 \<noteq> None"
+              using c2 wellFormed_callOrigin_dom3 by blast
+
+            have [simp]: "commitedCalls S' = dom (calls S')"
+            proof (rule commitedCalls_simps)
+              show "\<And>tx. tx \<in> Option.these (range (callOrigin S')) \<Longrightarrow> transactionStatus S' tx \<noteq> Some Uncommited"
+                by (metis c15 image_iff in_these_eq no_uncommitted)
+
+              show "state_wellFormed S'"
+                by simp
+            qed
 
             show "Option.these (range (callOrigin S')) \<subseteq> insert t (dom (transactionStatus S'))"
               by (simp add: subset_insertI2)
@@ -905,739 +992,142 @@ proof (rule show_correctness_via_single_session)
             from `invariant_all S'`
             have oldInv: "inv (invContextVis S' vis)" if "consistentSnapshot S' vis" for vis
               by (auto simp add: invariant_all_def that)
-            have "inv (invContextVis S' (visa - {c,ca}))"
+            have oldInv_visa: "inv (invContextVis S' (visa - {c,ca}))"
             proof (rule oldInv)
+
+
               from c14
               show "consistentSnapshot S' (visa - {c, ca})"
               proof (auto simp add: consistentSnapshotH_def)
 
-                show "causallyConsistent (updateHb (happensBefore S') vis [c, ca]) visa  \<Longrightarrow> causallyConsistent (happensBefore S') (visa - {c, ca})"
+                show "causallyConsistent (updateHb (happensBefore S') vis [c, ca]) visa  
+                  \<Longrightarrow> causallyConsistent (happensBefore S') (visa - {c, ca})"
                   apply (auto simp add: causallyConsistent_def updateHb_cons)
                   using c2 c8 wellFormed_happensBefore_calls_l apply blast
                   using c12 c2 wellFormed_happensBefore_calls_l by blast
 
 
-
-                (* TODO this should be done automatically, since it will be needed every time *)
-                find_theorems consistentSnapshot 
+                show "transactionConsistent (callOrigin S'(c \<mapsto> t, ca \<mapsto> t)) (transactionStatus S'(t \<mapsto> Commited)) visa
+                  \<Longrightarrow> transactionConsistent (callOrigin S') (transactionStatus S') (visa - {c, ca})"
+                  apply (subst  transactionConsistent_def)
+                  by (auto simp add: visa_callOrigin c15 elim!:  transactionConsistent_all_from_same dest!:transactionConsistent_Commited split: if_splits)
 
               qed
+            qed
 
             show "example_chat.inv
-               \<lparr>calls = calls S'(c \<mapsto> Call ''message_exists'' [MessageId mId] (Bool True), ca \<mapsto> Call ''message_content_assign'' [MessageId mId, ls_content lsInit] Undef),
+               \<lparr>calls = calls S'(c \<mapsto> Call message_exists [MessageId mId] (Bool True), ca \<mapsto> Call message_content_assign [MessageId mId, ls_content lsInit] Undef),
                   happensBefore = updateHb (happensBefore S') vis [c, ca], i_visibleCalls = visa, i_callOrigin = callOrigin S'(c \<mapsto> t, ca \<mapsto> t), i_transactionOrigin = transactionOrigin S',
                   i_knownIds = knownIds S', i_invocationOp = invocationOp S', i_invocationRes = invocationRes S'\<rparr>" (is "inv ?state")
             proof (cases "{c,ca} \<subseteq> visa")
+              case False
+              with c14
+              have [simp]: "c \<notin> visa" and [simp]: "ca \<notin> visa" (* all or nothing *)
+                 apply (auto simp add: consistentSnapshotH_def )
+                 apply (smt fun_upd_other fun_upd_same transactionConsistent_def)
+                apply (smt fun_upd_other fun_upd_same transactionConsistent_def)
+                done
+
+              hence "visa - {ca} = visa" and [simp]: "visa - {c} = visa"
+                by auto
+              hence "visa - {c,ca} = visa"
+                by blast
+              have [simp]: "dom (calls S') \<inter> visa = visa"
+                using visa'_subset by auto 
+
+              have hb_restrict_simps:  "(c1, c2) \<in> happensBefore S' |r visa \<longleftrightarrow> c1 \<in> visa \<and> c2 \<in> visa \<and> (c1, c2) \<in> happensBefore S'" for c1 c2
+                by (auto simp add: restrict_relation_def)
+
+              have updateHb_restrict_simps: "updateHb (happensBefore S') vis [c, ca] |r visa = happensBefore S' |r visa"
+                by (auto simp add: updateHb_cons restrict_relation_def)
+
+
+
+              have "inv (invContextVis S' (visa))"
+                using oldInv_visa by auto
+              thus "inv ?state"
+              proof (auto simp add: inv_def )
+                assume "inv1 (invContextVis S' visa)"
+                  and "inv2 (invContextVis S' visa)"
+                  and "inv2_h1 (invContextVis S' visa)"
+
+                from `inv1 (invContextVis S' visa)`
+                show "inv1 ?state"
+                  by (auto simp add: inv1_def mkContext_def  hb_restrict_simps updateHb_restrict_simps)
+
+                from `inv2 (invContextVis S' visa)`
+                show "inv2 ?state"
+                  by (auto simp add: inv2_def mkContext_def hb_restrict_simps updateHb_restrict_simps)
+
+                from `inv2_h1 (invContextVis S' visa)` 
+                  and `crdtSpec message_exists [MessageId mId] (getContextH (calls S') (happensBefore S') (Some vis)) (Bool True)`
+                show "inv2_h1 ?state"
+                  apply (auto simp add: inv2_h1_def mkContext_def hb_restrict_simps updateHb_restrict_simps crdtSpec_def crdtSpec_message_exists_def 
+                       crdtSpec_message_exists_h_def getContextH_def callsWithOpArgsH_def
+                       updateHb_cons message_updates_def)
+                  using c12 c2 wellFormed_happensBefore_calls_r by blast
+              qed
+
+            next
               case True
               hence [simp]: "c\<in>visa" and [simp]: "ca\<in>visa"
                 by auto
 
-              find_theorems "inv"
+              from c14
+              have vis_subset_visa: "c1\<in>visa" if "c1\<in>vis" for c1
+                 apply (auto simp add: consistentSnapshotH_def causallyConsistent_def updateHb_cons)
+                using \<open>c \<in> visa\<close> that by blast
+
+              from oldInv_visa
+              have "inv1 (invContextVis S' (visa - {c,ca}))"
+                  and "inv2 (invContextVis S' (visa - {c,ca}))"
+                  and "inv2_h1 (invContextVis S' (visa - {c,ca}))"
+                by (auto simp add: inv_def)
 
               show ?thesis 
               proof (auto simp add: inv_def)
+                from `inv1 (invContextVis S' (visa - {c,ca}))`
                 show "inv1 ?state"
-                  apply (auto simp add: inv1_def mkContext_def crdtSpec_chat_contains_h_def crdtSpec_message_exists_h_def callsWithOpArgsH_update_simps)
+                  apply (auto simp add: inv1_def mkContext_def crdtSpec_chat_contains_h_def crdtSpec_message_exists_h_def  
+                        restrict_relation_def message_updates_def callsWithOpArgsH_def updateHb_cons dom_exists
+                        cong: conj_cong)
+                   by metis+
+
+                 (*from `inv2 (invContextVis S' (visa - {c,ca}))`*)
+                 show "inv2 ?state"
+                 proof (auto simp add: inv2_def)
+                   fix m
+                   assume "crdtSpec_message_exists_h [m] (mkContext \<lparr>calls = calls S'(c \<mapsto> Call message_exists [MessageId mId] (Bool True), ca \<mapsto> Call message_content_assign [MessageId mId, ls_content lsInit] Undef),
+                        happensBefore = updateHb (happensBefore S') vis [c, ca], i_visibleCalls = visa, i_callOrigin = callOrigin S'(c \<mapsto> t, ca \<mapsto> t),
+                        i_transactionOrigin = transactionOrigin S', i_knownIds = knownIds S', i_invocationOp = invocationOp S', i_invocationRes = invocationRes S'\<rparr>)"
+
+                   
+
+                   with `crdtSpec message_exists [MessageId mId] (getContextH (calls S') (happensBefore S') (Some vis)) (Bool True)`
+                   have m_ex: "crdtSpec_message_exists_h [m] (mkContext (invContextVis S' (visa - {c, ca})))"
+                     by (auto simp add: crdtSpec_def crdtSpec_message_exists_def  getContextH_def crdtSpec_message_exists_h_def message_updates_def callsWithOpArgsH_def dest: vis_subset_visa split: if_splits)
+
+                   from this obtain a where "crdtSpec_message_author_read [m] (mkContext (invContextVis S' (visa - {c, ca}))) (ListVal [a])"
+                     using `inv2 (invContextVis S' (visa - {c,ca}))` by (auto simp  add: inv2_def)
+
+                   from this
+                   have "crdtSpec_message_author_read [m]
+                      (mkContext \<lparr>calls = calls S'(c \<mapsto> Call message_exists [MessageId mId] (Bool True), ca \<mapsto> Call message_content_assign [MessageId mId, ls_content lsInit] Undef),
+                                    happensBefore = updateHb (happensBefore S') vis [c, ca], i_visibleCalls = visa, i_callOrigin = callOrigin S'(c \<mapsto> t, ca \<mapsto> t),
+                                    i_transactionOrigin = transactionOrigin S', i_knownIds = knownIds S', i_invocationOp = invocationOp S', i_invocationRes = invocationRes S'\<rparr>)
+                      (ListVal [a])"
+                     apply (auto simp add: crdtSpec_message_author_read_def callsWithOpArgsH_def callsOfOpH_def restrict_relation_def dom_exists)
+                     apply (auto simp add:  updateHb_cons)
+                     done
+
+
+                     from this
+                   show "\<exists>a. crdtSpec_message_author_read [m]
+                      (mkContext \<lparr>calls = calls S'(c \<mapsto> Call message_exists [MessageId mId] (Bool True), ca \<mapsto> Call message_content_assign [MessageId mId, ls_content lsInit] Undef),
+                                    happensBefore = updateHb (happensBefore S') vis [c, ca], i_visibleCalls = visa, i_callOrigin = callOrigin S'(c \<mapsto> t, ca \<mapsto> t),
+                                    i_transactionOrigin = transactionOrigin S', i_knownIds = knownIds S', i_invocationOp = invocationOp S', i_invocationRes = invocationRes S'\<rparr>)
+                      (ListVal [a])"
+                     apply auto
 
-
-                  find_theorems callsWithOpArgsH
-                  apply (clarsimp simp add: inv1_def mkContext_def operationContext.simps invariantContext.simps crdtSpec_chat_contains_h_def crdtSpec_message_exists_h_def  restrict_fun_upd)
-              qed
-            next
-              case False
-              then show ?thesis sorry
-            qed
-
-
-            proof (auto simp add: inv_def)
-              show "inv1 ?state"
-                apply (simp only: inv1_def mkContext_def operationContext.simps invariantContext.simps)
-                apply (clarsimp simp del: restrict_fun_upd)
-                (*using [[simp_trace]]*)
-                apply (subst crdtSpec_message_exists_h_def2)
-                apply ( simp del: restrict_fun_upd)
-                (* apply (auto simp add:  crdtSpec_message_exists_h_def del: restrict_fun_upd split: if_splits)*)
-
-                apply (subst restrict_fun_upd)+
-                apply (subst(asm) restrict_fun_upd)+
-
-                find_theorems i_visibleCalls
-                apply clarify
-                sorry
-
-              show "inv2 ?state"
-                sorry
-
-              show "inv2_h1 ?state"
-                sorry
-
-
-
-          proof (auto simp add: inv_def)
-            have [simp]: "prog S' = progr"
-              by (simp add: c3)
-
-
-            hence no_calls_in_t: "callOrigin S' c \<noteq> Some t" for c
-              using c15 by blast
-
-            have "consistentSnapshot S' (visa - {c,ca})"
-              apply (rule consistentSnapshot_subset[OF c14], auto)
-              using c2 c8 wellFormed_happensBefore_calls_l apply blast
-              using c12 c2 wellFormed_happensBefore_calls_l apply blast
-              using c2 c8 wellFormed_callOrigin_dom2 apply blast
-                apply (simp add: c12 c2)
-              using no_calls_in_t apply blast
-              by (simp add: c2 domD domI )
-
-
-
-            find_theorems name: consistentSnapshot
-
-            with `invariant_all S'` 
-            have oldInv: "inv (invContextVis S' (visa - {c,ca}))"
-              by (auto simp add: invariant_all_def)
-            hence old_inv1: "inv1 (invContextVis S' (visa - {c, ca}))"
-              and  old_inv2: "inv2 (invContextVis S' (visa - {c, ca}))"
-              and old_inv2_h1: "inv2_h1 (invContextVis S' (visa - {c, ca}))"
-              by (auto simp add: inv_def)
-
-            thm c14 
-
-            have domEq[simp]: "dom (callOrigin S') = dom (calls S')"
-              by (simp add: c2)
-
-            have "insert ca (insert c (dom (callOrigin S'))) = insert ca (insert c (dom (calls S')))"
-              by simp
-
-            thm invContextH_update_calls
-
-
-            have [simp]: "c \<noteq> ca"
-              using c11 by blast 
-
-            
-
-            show "inv1 (invContextH (callOrigin S'(c \<mapsto> t, ca \<mapsto> t)) (transactionOrigin S') (transactionStatus S'(t \<mapsto> Commited)) (updateHb (happensBefore S') vis [c, ca])
-               (calls S'(c \<mapsto> Call ''message_exists'' [MessageId mId] (Bool True), ca \<mapsto> Call ''message_content_assign'' [MessageId mId, ls_content lsInit] Undef)) (knownIds S')
-               (invocationOp S') (invocationRes S') (Some visa))"
-              apply (auto simp add: inv1_def)
-              apply (subst crdtSpec_message_exists_h_def2)
-              apply (auto simp add: is_message_update_simps cong: conj_cong)
-                     apply (auto simp add: crdtSpec_chat_contains_h_def callsWithOpArgs_simps split: if_splits cong: conj_cong)
-
-
-              apply (subst(asm) callsWithOpArgs_simps)
-              apply simp
-                apply simp
-              apply simp
-              using c2 domD apply fastforc
-                apply auto[1]
-
-
-            proof (auto simp add: inv1_def)
-              fix cb m
-              assume a0: "crdtSpec_chat_contains_h [cb, m]
-                       (mkContext
-                         (invContextH (callOrigin S'(c \<mapsto> t, ca \<mapsto> t)) (transactionOrigin S') (transactionStatus S'(t \<mapsto> Commited))
-                           (updateHb (happensBefore S') vis [c, ca])
-                           (calls S'(c \<mapsto> Call ''message_exists'' [MessageId mId] (Bool True), ca \<mapsto> Call ''message_content_assign'' [MessageId mId, ls_content lsInit] Undef))
-                           (knownIds S') (invocationOp S') (invocationRes S') (Some visa)))"
-
-
-
-(*
- \<lbrakk>\<forall>cr. isCommittedH (callOrigin S'(c \<mapsto> t, ca \<mapsto> t)) (transactionStatus S'(t \<mapsto> Commited)) cr \<longrightarrow>
-                   cr \<in> visa \<longrightarrow>
-                   calls S' cr \<triangleq> Call ''chat_remove'' [cb, m] Undef \<longrightarrow>
-                   cr = c \<or> cr = ca \<or> (\<exists>caa. caa \<noteq> c \<and>
-                                              (caa = c \<or>
-                                               caa \<noteq> ca \<and>
-                                               (caa = ca \<or>
-                                                isCommittedH (callOrigin S'(c \<mapsto> t, ca \<mapsto> t)) (transactionStatus S'(t \<mapsto> Commited)) caa \<and>
-                                                caa \<in> visa \<and>
-                                                (cr = c \<and> caa = ca \<or> (cr, caa) \<in> happensBefore S' \<or> cr \<in> vis \<and> caa = c \<or> cr \<in> vis \<and> caa = ca) \<and>
-                                                calls S' caa \<triangleq> Call ''chat_add'' [cb, m] Undef)));
-              ; ; ; 
-              \<rbrakk>
-*)
-
-              have commitedCallsH_t_simp: "commitedCallsH (callOrigin S') (transactionStatus S'(t \<mapsto> Commited)) 
-                  = commitedCalls S'"
-                apply (auto simp add: commitedCallsH_def isCommittedH_def)
-                using no_calls_in_t by blast
-
-
-              have isCommittedH_simp1: "isCommittedH (callOrigin S'(c \<mapsto> t, ca \<mapsto> t)) (transactionStatus S'(t \<mapsto> Commited)) cx" if "calls S' cx \<triangleq> someCall" for cx someCall
-                apply (auto simp add: isCommittedH_def)
-                by (metis (full_types) c2 domIff no_uncommitted not_Some_eq that transactionStatus.exhaust wellFormed_callOrigin_dom wellFormed_state_callOrigin_transactionStatus)
-
-
-              find_theorems "calls S' ca"
-
-              find_theorems invContextH 
-              find_theorems name: cong "op\<longrightarrow>"
-
-              have notC: "cr \<noteq> c" if "calls S' cr \<triangleq> someCall" for cr someCall
-                using that `calls S' c = None` by auto 
-              have notCa: "cr \<noteq> ca" if "calls S' cr \<triangleq> someCall" for cr someCall
-                using that `calls S' ca = None` by auto 
-
-              from a0 have ???
-                apply (auto simp add: crdtSpec_chat_contains_h_def mkContext_simps commitedCallsH_true split: if_splits)
-                apply (simp_all add: commitedCallsH_simp commitedCallsH_t_simp notC notCa cong: conj_cong imp_cong)
-                     apply (auto simp add: `calls S' ca = None` `calls S' c = None` )[1]
-                sorry
-
-              from a0 obtain c_add 
-                where [simp]: "c_add \<noteq> c"
-                  and [simp]: "c_add \<noteq> ca"
-                  and cc3: "calls S' c_add \<triangleq> Call ''chat_add'' [cb, m] Undef"
-                  and cc2: "c_add \<in> visa"
-                  and cc1: "isCommittedH (callOrigin S'(c \<mapsto> t, ca \<mapsto> t)) (transactionStatus S'(t \<mapsto> Commited)) c_add"
-                  and cc4: "\<forall>cr. isCommittedH (callOrigin S'(c \<mapsto> t, ca \<mapsto> t)) (transactionStatus S'(t \<mapsto> Commited)) cr \<longrightarrow>
-                   cr \<in> visa \<longrightarrow>
-                   calls S' cr \<triangleq> Call ''chat_remove'' [cb, m] Undef \<longrightarrow>
-                   cr = c \<or> cr = ca \<or> (\<exists>caa. caa \<noteq> c \<and>
-                                              (caa = c \<or>
-                                               caa \<noteq> ca \<and>
-                                               (caa = ca \<or>
-                                                isCommittedH (callOrigin S'(c \<mapsto> t, ca \<mapsto> t)) (transactionStatus S'(t \<mapsto> Commited)) caa \<and>
-                                                caa \<in> visa \<and>
-                                                (cr = c \<and> caa = ca \<or> (cr, caa) \<in> happensBefore S' \<or> cr \<in> vis \<and> caa = c \<or> cr \<in> vis \<and> caa = ca) \<and>
-                                                calls S' caa \<triangleq> Call ''chat_add'' [cb, m] Undef)))"
-apply (auto simp add: crdtSpec_chat_contains_h_def mkContext_simps commitedCallsH_true isCommittedH_simp1 split: if_splits)
-                     apply (simp_all add: commitedCallsH_simp commitedCallsH_t_simp  notC notCa isCommittedH_simp1  cong: conj_cong imp_cong)
-                     apply atomize_elim
-                     apply (rule_tac x=" caa" in exI)
-                     apply safe[1]
-                apply (smt commitedCallsH_def fun_upd_apply isCommittedH_def mem_Collect_eq)
-                     apply (drule_tac x=cr in spec)
-                     apply safe[1]
-                apply (smt c12 c8 commitedCallsH_t_simp commitedCallsH_true domI domIff fun_upd_other isCommittedH_def)
-
-
-
-                sorry
-
-              hence "crdtSpec_chat_contains_h [cb, m] (mkContext (invContextVis S' (visa - {c, ca})))"
-                apply (auto simp add: crdtSpec_chat_contains_h_def mkContext_simps)
-                apply (rule_tac x=c_add in exI)
-                apply (auto simp add: cc2 cc3)
-                using cc1 apply (auto simp add: isCommittedH_def no_calls_in_t split: if_splits)
-                apply (drule_tac x=cr in spec)
-                apply auto
-                using no_calls_in_t by blast
-
-              with old_inv1
-              have "crdtSpec_message_exists_h [m] (mkContext (invContextVis S' (visa - {c, ca})))"
-                by (auto simp add: inv1_def)
-
-              thus "crdtSpec_message_exists_h [m]
-             (mkContext (invContextH (callOrigin S'(c \<mapsto> t, ca \<mapsto> t)) (transactionOrigin S') (transactionStatus S'(t \<mapsto> Commited))
-                          (updateHb (happensBefore S') vis [c, ca])
-                          (calls S'(c \<mapsto> Call ''message_exists'' [MessageId mId] (Bool True), ca \<mapsto> Call ''message_content_assign'' [MessageId mId, ls_content lsInit] resa))
-                          (knownIds S') (invocationOp S') (invocationRes S') (Some visa)))"
-                apply (auto simp add: crdtSpec_message_exists_h_def mkContext_simps is_message_update_vis_simps)
-                 apply (auto simp add: is_message_updateH_def isCommittedH_def split: option.splits)
-                 apply fastforce
-                by (metis no_calls_in_t)
-            qed
-
-            show "inv2 (invContextH (callOrigin S'(c \<mapsto> t, ca \<mapsto> t)) (transactionOrigin S') (transactionStatus S'(t \<mapsto> Commited)) (updateHb (happensBefore S') vis [c, ca])
-           (calls S'(c \<mapsto> Call ''message_exists'' [MessageId mId] (Bool True), ca \<mapsto> Call ''message_content_assign'' [MessageId mId, ls_content lsInit] resa)) (knownIds S')
-           (invocationOp S') (invocationRes S') (Some visa))"
-            proof (auto simp add: inv2_def)
-              fix m
-              assume a_message_exists: "crdtSpec_message_exists_h [m]
-          (mkContext (invContextH (callOrigin S'(c \<mapsto> t, ca \<mapsto> t)) (transactionOrigin S') (transactionStatus S'(t \<mapsto> Commited))
-                       (updateHb (happensBefore S') vis [c, ca])
-                       (calls S'(c \<mapsto> Call ''message_exists'' [MessageId mId] (Bool True), ca \<mapsto> Call ''message_content_assign'' [MessageId mId, ls_content lsInit] resa))
-                       (knownIds S') (invocationOp S') (invocationRes S') (Some visa)))"
-
-
-              {
-                assume [simp]: "m = MessageId mId" and "vis \<subseteq> visa"
-                from `crdtSpec ''message_exists'' [MessageId mId] (getContextH (calls S') (happensBefore S') (Some vis)) (Bool True)`
-                have "crdtSpec_message_exists_h [m] (mkContext (invContextVis S' (visa - {c, ca})))"
-                  apply (auto simp add: crdtSpec_def crdtSpec_message_exists_def crdtSpec_message_exists_h_def mkContext_simps is_message_update_vis_simps)
-
-                   apply (auto simp add: is_message_updateH_simp isCommittedH_def  split: option.splits if_splits)
-                   apply (rule_tac x=cb in exI)
-                   apply (rule_tac x=x2 in exI)
-                   apply (auto simp add: getContextH_def restrict_map_def split: option.splits if_splits)[1]
-                      apply (metis c10 c15 c2 c6 domIff not_None_eq wellFormed_callOrigin_dom wellFormed_state_transaction_consistent(1))(* TODO general*)
-                  using \<open>vis \<subseteq> visa\<close> apply auto[1]
-                    apply (simp add: `calls S' c = None`)
-                   apply (simp add: `calls S' ca = None`) 
-                  apply (auto simp add: getContextH_def restrict_map_def split: option.splits if_splits)[1]
-                  sorry
-              }
-
-
-              show "\<exists>a. crdtSpec_message_author_read [m]
-              (mkContext (invContextH (callOrigin S'(c \<mapsto> t, ca \<mapsto> t)) (transactionOrigin S') (transactionStatus S'(t \<mapsto> Commited))
-                           (updateHb (happensBefore S') vis [c, ca])
-                           (calls S'(c \<mapsto> Call ''message_exists'' [MessageId mId] (Bool True), ca \<mapsto> Call ''message_content_assign'' [MessageId mId, ls_content lsInit] resa))
-                           (knownIds S') (invocationOp S') (invocationRes S') (Some visa)))
-              (ListVal [a])"
-                sorry
-            qed
-
-
-            show "inv2_h1 (invContextH (callOrigin S'(c \<mapsto> t, ca \<mapsto> t)) (transactionOrigin S') (transactionStatus S'(t \<mapsto> Commited)) (updateHb (happensBefore S') vis [c, ca])
-              (calls S'(c \<mapsto> Call ''message_exists'' [MessageId mId] (Bool True), ca \<mapsto> Call ''message_content_assign'' [MessageId mId, ls_content lsInit] resa)) (knownIds S')
-              (invocationOp S') (invocationRes S') (Some visa))"
-              sorry
-
-          qed
-
-          text {* editMessage, case message does exist, return from procedure  *}
-          show "example_chat.inv (invContextH (callOrigin S'(c \<mapsto> t, ca \<mapsto> t)) (transactionOrigin S') (transactionStatus S'(t \<mapsto> Commited)) (updateHb (happensBefore S') vis [c, ca]) (calls S'(c \<mapsto> Call ''message_exists'' [MessageId mId] (Bool True), ca \<mapsto> Call ''message_content_assign'' [MessageId mId, ls_content lsInit] resa)) (knownIds S' \<union> uniqueIds Undef) (invocationOp S') (invocationRes S'(i \<mapsto> Undef)) (Some visa))"
-            if c0: "transactionStatus S t = None"
-              and c1: "invariant_all S'"
-              and c2: "state_wellFormed S'"
-              and c3: "state_monotonicGrowth S S'"
-              and c4: "localState S' i \<triangleq> lsInit\<lparr>ls_id := MessageId mId, ls_pc := Suc 0\<rparr>"
-              and c5: "currentProc S' i \<triangleq> editMessageImpl"
-              and c6: "currentTransaction S' i \<triangleq> t"
-              and c7: "transactionOrigin S' t \<triangleq> i"
-              and c8: "\<forall>c. callOrigin S' c \<noteq> Some t"
-              and c9: "calls S' c = None"
-              and c10: "crdtSpec ''message_exists'' [MessageId mId] (getContextH (calls S') (happensBefore S') (Some vis)) (Bool True)"
-              and c11: "visibleCalls S' i \<triangleq> vis"
-              and c12: "ca \<noteq> c"
-              and c13: "calls S' ca = None"
-              and c15: "consistentSnapshot (S'\<lparr>calls := calls S'(c \<mapsto> Call ''message_exists'' [MessageId mId] (Bool True), ca \<mapsto> Call ''message_content_assign'' [MessageId mId, ls_content lsInit] resa), callOrigin := callOrigin S'(c \<mapsto> t, ca \<mapsto> t), happensBefore := updateHb (happensBefore S') vis [c, ca], currentTransaction := (currentTransaction S')(i := None), transactionStatus := transactionStatus S'(t \<mapsto> Commited), localState := (localState S')(i := None), currentProc := (currentProc S')(i := None), visibleCalls := (visibleCalls S')(i := None), invocationRes := invocationRes S'(i \<mapsto> Undef), knownIds := knownIds S' \<union> uniqueIds Undef\<rparr>) visa"
-            for  t S' c vis ca resa visa
-          proof -
-            from c15
-            have c15': "consistentSnapshot (S'\<lparr>calls := calls S'(c \<mapsto> Call ''message_exists'' [MessageId mId] (Bool True), ca \<mapsto> Call ''message_content_assign'' [MessageId mId, ls_content lsInit] resa), callOrigin := callOrigin S'(c \<mapsto> t, ca \<mapsto> t), visibleCalls := visibleCalls S'(i \<mapsto> insert ca (insert c vis)), happensBefore := updateHb (happensBefore S') vis [c, ca], localState := localState S'(i \<mapsto> lsInit\<lparr>ls_id := MessageId mId, ls_pc := 4\<rparr>), currentTransaction := (currentTransaction S')(i := None), transactionStatus := transactionStatus S'(t \<mapsto> Commited)\<rparr>) visa"
-              by (auto simp add: consistentSnapshot_def)
-
-            from h[OF c0 c1 c2 c3 c4 c5 c6 c7 c9 c10 c11 c12 c13 c15' c8]
-            show "example_chat.inv (invContextH (callOrigin S'(c \<mapsto> t, ca \<mapsto> t)) (transactionOrigin S') (transactionStatus S'(t \<mapsto> Commited)) (updateHb (happensBefore S') vis [c, ca]) (calls S'(c \<mapsto> Call ''message_exists'' [MessageId mId] (Bool True), ca \<mapsto> Call ''message_content_assign'' [MessageId mId, ls_content lsInit] resa)) (knownIds S' \<union> uniqueIds Undef) (invocationOp S') (invocationRes S'(i \<mapsto> Undef)) (Some visa))"
-              by (meson example_chat.inv_def inv1_unchanged inv2_h1_unchanged inv2_unchanged)
-          qed
-
-          text {* editMessage, case message does not exist  *}
-          show h: "example_chat.inv (invContextH (callOrigin S'(c \<mapsto> t)) (transactionOrigin S') (transactionStatus S'(t \<mapsto> Commited)) (happensBefore S' \<union> vis \<times> {c}) (calls S'(c \<mapsto> Call ''message_exists'' [MessageId mId] res)) (knownIds S') (invocationOp S') (invocationRes S') (Some visa))"
-            if c0: "transactionStatus S t = None"
-              and c1: "invariant_all S'"
-              and c2: "state_wellFormed S'"
-              and c3: "state_monotonicGrowth S S'"
-              and c4: "localState S' i \<triangleq> lsInit\<lparr>ls_id := MessageId mId, ls_pc := Suc 0\<rparr>"
-              and c5: "currentProc S' i \<triangleq> editMessageImpl"
-              and c6: "currentTransaction S' i \<triangleq> t"
-              and c7: "transactionOrigin S' t \<triangleq> i"
-              and c8: "\<forall>c. callOrigin S' c \<noteq> Some t"
-              and c9: "res \<noteq> Bool True"
-              and c10: "calls S' c = None"
-              and c11: "crdtSpec ''message_exists'' [MessageId mId] (getContextH (calls S') (happensBefore S') (Some vis)) res"
-              and c12: "visibleCalls S' i \<triangleq> vis"
-              and c13: "consistentSnapshot (S'\<lparr>calls := calls S'(c \<mapsto> Call ''message_exists'' [MessageId mId] res), callOrigin := callOrigin S'(c \<mapsto> t), visibleCalls := visibleCalls S'(i \<mapsto> insert c vis), happensBefore := happensBefore S' \<union> vis \<times> {c}, localState := localState S'(i \<mapsto> lsInit\<lparr>ls_id := MessageId mId, ls_pc := 4\<rparr>), currentTransaction := (currentTransaction S')(i := None), transactionStatus := transactionStatus S'(t \<mapsto> Commited)\<rparr>) visa"
-            for  t S' c res vis visa
-          proof -
-            have [simp]: "prog S' = progr"
-              by (simp add: c3)
-
-
-            hence no_calls_in_t: "callOrigin S' c \<noteq> Some t" for c
-              by (simp add: c8)
-
-            have "consistentSnapshot S' (visa - {c})"
-              apply (rule consistentSnapshot_subset[OF c13], auto)
-              using c10 c2 wellFormed_happensBefore_calls_l apply blast
-              using c10 c2 wellFormed_callOrigin_dom2 apply blast
-              using no_calls_in_t apply blast
-              by (simp add: c2 domD domI wellFormed_callOrigin_dom)
-
-
-            with `invariant_all S'` 
-            have oldInv: "inv (invContextVis S' (visa - {c}))"
-              by (auto simp add: invariant_all_def)
-            hence old_inv1: "inv1 (invContextVis S' (visa - {c}))"
-              and  old_inv2: "inv2 (invContextVis S' (visa - {c}))"
-              and old_inv2_h1: "inv2_h1 (invContextVis S' (visa - {c}))"
-              by (auto simp add: inv_def)
-
-            show ?thesis
-            proof (auto simp add: inv_def)
-              show " inv1 (invContextH (callOrigin S'(c \<mapsto> t)) (transactionOrigin S') (transactionStatus S'(t \<mapsto> Commited)) (happensBefore S' \<union> vis \<times> {c})
-                 (calls S'(c \<mapsto> Call ''message_exists'' [MessageId mId] res)) (knownIds S') (invocationOp S') (invocationRes S') (Some visa))"
-              proof (auto simp add: inv1_def)
-                fix ca m
-                assume "crdtSpec_chat_contains_h [ca, m]
-             (mkContext (invContextH (callOrigin S'(c \<mapsto> t)) (transactionOrigin S') (transactionStatus S'(t \<mapsto> Commited)) (happensBefore S' \<union> vis \<times> {c})
-                          (calls S'(c \<mapsto> Call ''message_exists'' [MessageId mId] res)) (knownIds S') (invocationOp S') (invocationRes S') (Some visa)))"
-
-(*
-\<And>c_add. \<lbrakk>\<forall>cr. calls S' cr \<triangleq> Call ''chat_remove'' [ca, m] Undef \<longrightarrow>
-                   cr \<in> visa \<longrightarrow>
-                   isCommittedH (callOrigin S'(c \<mapsto> t)) (transactionStatus S'(t \<mapsto> Commited)) cr \<longrightarrow>
-                   cr = c \<or>
-                   (\<exists>caa. caa \<noteq> c \<and>
-                          (caa = c \<or>
-                           isCommittedH (callOrigin S'(c \<mapsto> t)) (transactionStatus S'(t \<mapsto> Commited)) caa \<and>
-                           caa \<in> visa \<and> ((cr, caa) \<in> happensBefore S' \<or> cr \<in> vis \<and> caa = c) \<and> calls S' caa \<triangleq> Call ''chat_add'' [ca, m] Undef));
-              ; ; ; \<rbrakk>
-*)
-
-                from this obtain c_add 
-                  where cc4: "c_add \<noteq> c"
-                    and cc3: "calls S' c_add \<triangleq> Call ''chat_add'' [ca, m] Undef"
-                    and cc2: "c_add \<in> visa"
-                    and cc1: "isCommittedH (callOrigin S'(c \<mapsto> t)) (transactionStatus S'(t \<mapsto> Commited)) c_add"
-                    and cc5: "\<forall>cr. calls S' cr \<triangleq> Call ''chat_remove'' [ca, m] Undef \<longrightarrow>
-                         cr \<in> visa \<longrightarrow>
-                         isCommittedH (callOrigin S'(c \<mapsto> t)) (transactionStatus S'(t \<mapsto> Commited)) cr \<longrightarrow>
-                         cr = c \<or>
-                         (\<exists>caa. caa \<noteq> c \<and>
-                                (caa = c \<or>
-                                 isCommittedH (callOrigin S'(c \<mapsto> t)) (transactionStatus S'(t \<mapsto> Commited)) caa \<and>
-                                 caa \<in> visa \<and> ((cr, caa) \<in> happensBefore S' \<or> cr \<in> vis \<and> caa = c) \<and> calls S' caa \<triangleq> Call ''chat_add'' [ca, m] Undef))"
-                  by (auto simp add: crdtSpec_chat_contains_h_def mkContext_simps split: if_splits)
-
-
-                hence "crdtSpec_chat_contains_h [ca, m] (mkContext (invContextVis S' (visa - {c})))"
-                  apply (auto simp add: crdtSpec_chat_contains_h_def mkContext_simps)
-                  apply (rule_tac x=c_add in exI)
-                  apply (auto simp add: cc2 cc3)
-                  using cc1 apply (auto simp add: isCommittedH_def no_calls_in_t split: if_splits)
-                  apply (drule_tac x=cr in spec)
-                  apply auto
-                  using c8 by blast
-
-                with old_inv1
-                have "crdtSpec_message_exists_h [m] (mkContext (invContextVis S' (visa - {c})))"
-                  by (auto simp add: inv1_def)
-
-                thus "crdtSpec_message_exists_h [m]
-                   (mkContext (invContextH (callOrigin S'(c \<mapsto> t)) (transactionOrigin S') (transactionStatus S'(t \<mapsto> Commited)) (happensBefore S' \<union> vis \<times> {c})
-                                (calls S'(c \<mapsto> Call ''message_exists'' [MessageId mId] res)) (knownIds S') (invocationOp S') (invocationRes S') (Some visa)))"
-                  apply (auto simp add: crdtSpec_message_exists_h_def mkContext_simps is_message_update_vis_simps)
-                   apply (auto simp add: is_message_updateH_def isCommittedH_def split: option.splits)
-                   apply fastforce
-                  by (metis no_calls_in_t)
-              qed
-
-              show "inv2 (invContextH (callOrigin S'(c \<mapsto> t)) (transactionOrigin S') (transactionStatus S'(t \<mapsto> Commited)) (happensBefore S' \<union> vis \<times> {c})
-           (calls S'(c \<mapsto> Call ''message_exists'' [MessageId mId] res)) (knownIds S') (invocationOp S') (invocationRes S') (Some visa))"
-                sorry
-
-              show "inv2_h1 (invContextH (callOrigin S'(c \<mapsto> t)) (transactionOrigin S') (transactionStatus S'(t \<mapsto> Commited)) (happensBefore S' \<union> vis \<times> {c})
-              (calls S'(c \<mapsto> Call ''message_exists'' [MessageId mId] res)) (knownIds S') (invocationOp S') (invocationRes S') (Some visa))"
-                sorry
-
-            qed
-
-          qed
-
-          text {* editMessage, case message does not exist, return from procedure  *}
-          show "example_chat.inv (invContextH (callOrigin S'(c \<mapsto> t)) (transactionOrigin S') (transactionStatus S'(t \<mapsto> Commited)) (happensBefore S' \<union> vis \<times> {c}) (calls S'(c \<mapsto> Call ''message_exists'' [MessageId mId] res)) (knownIds S' \<union> uniqueIds Undef) (invocationOp S') (invocationRes S'(i \<mapsto> Undef)) (Some visa))"
-            if c0: "transactionStatus S t = None"
-              and c1: "invariant_all S'"
-              and c2: "state_wellFormed S'"
-              and c3: "state_monotonicGrowth S S'"
-              and c4: "localState S' i \<triangleq> lsInit\<lparr>ls_id := MessageId mId, ls_pc := Suc 0\<rparr>"
-              and c5: "currentProc S' i \<triangleq> editMessageImpl"
-              and c6: "currentTransaction S' i \<triangleq> t"
-              and c7: "transactionOrigin S' t \<triangleq> i"
-              and c8: "\<forall>c. callOrigin S' c \<noteq> Some t"
-              and c9: "res \<noteq> Bool True"
-              and c10: "calls S' c = None"
-              and c11: "crdtSpec ''message_exists'' [MessageId mId] (getContextH (calls S') (happensBefore S') (Some vis)) res"
-              and c12: "visibleCalls S' i \<triangleq> vis"
-              and c13: "consistentSnapshot (S'\<lparr>calls := calls S'(c \<mapsto> Call ''message_exists'' [MessageId mId] res), callOrigin := callOrigin S'(c \<mapsto> t), happensBefore := happensBefore S' \<union> vis \<times> {c}, currentTransaction := (currentTransaction S')(i := None), transactionStatus := transactionStatus S'(t \<mapsto> Commited), localState := (localState S')(i := None), currentProc := (currentProc S')(i := None), visibleCalls := (visibleCalls S')(i := None), invocationRes := invocationRes S'(i \<mapsto> Undef), knownIds := knownIds S' \<union> uniqueIds Undef\<rparr>) visa"
-            for  t S' c res vis visa
-          proof -
-            from c13
-            have c13': "consistentSnapshot (S'\<lparr>calls := calls S'(c \<mapsto> Call ''message_exists'' [MessageId mId] res), callOrigin := callOrigin S'(c \<mapsto> t), visibleCalls := visibleCalls S'(i \<mapsto> insert c vis), happensBefore := happensBefore S' \<union> vis \<times> {c}, localState := localState S'(i \<mapsto> lsInit\<lparr>ls_id := MessageId mId, ls_pc := 4\<rparr>), currentTransaction := (currentTransaction S')(i := None), transactionStatus := transactionStatus S'(t \<mapsto> Commited)\<rparr>) visa"
-              by (auto simp add: consistentSnapshot_def)
-
-            from h[OF c0 c1 c2 c3 c4 c5 c6 c7 c8 c9 c10 c11 c12 c13']
-            show "example_chat.inv (invContextH (callOrigin S'(c \<mapsto> t)) (transactionOrigin S') (transactionStatus S'(t \<mapsto> Commited)) (happensBefore S' \<union> vis \<times> {c}) (calls S'(c \<mapsto> Call ''message_exists'' [MessageId mId] res)) (knownIds S' \<union> uniqueIds Undef) (invocationOp S') (invocationRes S'(i \<mapsto> Undef)) (Some visa))"
-              by (meson example_chat.inv_def inv1_unchanged inv2_h1_unchanged inv2_unchanged)
-          qed
-        qed
-      next
-
-        show "checkCorrectAll progr S i"
-          if c0: "invocationOp S i \<triangleq> (''deleteMessage'', [MessageId x4])"
-            and c1[simp]: "currentProc S i \<triangleq> deleteMessageImpl"
-            and c2[simp]: "localState S i \<triangleq> lsInit\<lparr>ls_id := MessageId x4\<rparr>"
-            and c3: "uniqueIdsInList [MessageId x4] \<subseteq> knownIds S"
-          for  x4
-        proof -
-          have progS[simp]: "prog S = progr"
-            using \<open>S \<in> initialStates progr i\<close> \<open>\<And>i S. S \<in> initialStates progr i \<Longrightarrow> prog S = progr\<close> by blast
-            
-          have sameProg[simp]: "prog S' = progr" if "state_monotonicGrowth S S'" for S'
-            using state_monotonicGrowth_prog that by force
-          have [simp]: "currentTransaction S i = None" 
-            using `S \<in> initialStates progr i`  initialStates_currentTransaction by blast 
-
-
-          from every_query_has_result
-
-          show "checkCorrectAll progr S i"
-          proof (auto simp add: checkCorrectAll_simps deleteMessageImpl_def; (subst invariant_all_def)?; auto? )
-
-            show "Ex (crdtSpec ''message_chat_read'' [MessageId x4] (getContext S' i))"
-              if c0: "transactionStatus S t = None"
-                and c1: "invariant_all S'"
-                and c2: "state_wellFormed S'"
-                and c3: "state_monotonicGrowth S S'"
-                and c4: "localState S' i \<triangleq> lsInit\<lparr>ls_id := MessageId x4, ls_pc := Suc 0\<rparr>"
-                and c5: "currentProc S' i \<triangleq> deleteMessageImpl"
-                and c6: "currentTransaction S' i \<triangleq> t"
-                and c7: "transactionOrigin S' t \<triangleq> i"
-                and c8: "\<forall>c. callOrigin S' c \<noteq> Some t"
-                and c9: "\<And>ctxt procName args. finite (dom (calls ctxt)) \<Longrightarrow> Ex (crdtSpec procName args ctxt)"
-              for  t S'
-              apply (rule every_query_has_result)
-              apply (auto simp add: getContextH_def split: option.split)
-              by (simp add: c2 wf_finite_calls)
-
-
-            show h: "example_chat.inv (invContextH (callOrigin S'(c \<mapsto> t, ca \<mapsto> t, cb \<mapsto> t)) (transactionOrigin S') (transactionStatus S'(t \<mapsto> Commited)) (insert (c, ca) (insert (ca, cb) (insert (c, cb) (happensBefore S' \<union> vis \<times> {c} \<union> vis \<times> {ca} \<union> vis \<times> {cb})))) (calls S'(c \<mapsto> Call ''message_chat_read'' [MessageId x4] res, ca \<mapsto> Call ''chat_remove'' [res, MessageId x4] Undef, cb \<mapsto> Call ''message_delete'' [MessageId x4] Undef)) (knownIds S') (invocationOp S') (invocationRes S') (Some visa))"
-              if c0: "transactionStatus S t = None"
-                and c1: "invariant_all S'"
-                and c2: "state_wellFormed S'"
-                and c3: "state_monotonicGrowth S S'"
-                and c4: "localState S' i \<triangleq> lsInit\<lparr>ls_id := MessageId x4, ls_pc := Suc 0\<rparr>"
-                and c5: "currentProc S' i \<triangleq> deleteMessageImpl"
-                and c6: "currentTransaction S' i \<triangleq> t"
-                and c7: "transactionOrigin S' t \<triangleq> i"
-                and c8: "\<forall>c. callOrigin S' c \<noteq> Some t"
-                and c9: "calls S' c = None"
-                and c10: "crdtSpec ''message_chat_read'' [MessageId x4] (getContextH (calls S') (happensBefore S') (Some vis)) res"
-                and c11: "visibleCalls S' i \<triangleq> vis"
-                and c12: "ca \<noteq> c"
-                and c13: "calls S' ca = None"
-                and c14: "cb \<noteq> c"
-                and c15: "cb \<noteq> ca"
-                and c16: "calls S' cb = None"
-                and c17: "\<And>ctxt procName args. finite (dom (calls ctxt)) \<Longrightarrow> Ex (crdtSpec procName args ctxt)"
-                and c18: "consistentSnapshot (S'\<lparr>calls := calls S'(c \<mapsto> Call ''message_chat_read'' [MessageId x4] res, ca \<mapsto> Call ''chat_remove'' [res, MessageId x4] Undef, cb \<mapsto> Call ''message_delete'' [MessageId x4] Undef), callOrigin := callOrigin S'(c \<mapsto> t, ca \<mapsto> t, cb \<mapsto> t), visibleCalls := visibleCalls S'(i \<mapsto> insert cb (insert ca (insert c vis))), happensBefore := insert (c, ca) (insert (ca, cb) (insert (c, cb) (happensBefore S' \<union> vis \<times> {c} \<union> vis \<times> {ca} \<union> vis \<times> {cb}))), localState := localState S'(i \<mapsto> lsInit\<lparr>ls_id := MessageId x4, ls_c := res, ls_pc := 5\<rparr>), currentTransaction := (currentTransaction S')(i := None), transactionStatus := transactionStatus S'(t \<mapsto> Commited)\<rparr>) visa"
-              for  t S' c res vis ca cb visa
-            proof (auto simp add: inv_def)
-              have [simp]: "prog S' = progr"
-                by (simp add: c3)
-
-
-              hence no_calls_in_t: "callOrigin S' c \<noteq> Some t" for c
-                using c8 by blast
-              
-              have "consistentSnapshot S' (visa - {c,ca,cb})"
-                apply (rule consistentSnapshot_subset[OF c18], auto)
-                using c2 c9 wellFormed_happensBefore_calls_l apply blast
-                using c13 c2 wellFormed_happensBefore_calls_l apply blast
-                using c16 c2 wellFormed_happensBefore_calls_l apply blast
-                    apply (simp add: c2 c9)
-                   apply (simp add: c13 c2)
-                using c16 c2 wellFormed_callOrigin_dom2 apply blast
-                using c8 apply auto[1]
-                by (simp add: c2 domD domI wellFormed_callOrigin_dom)
-              with `invariant_all S'` 
-              have oldInv: "inv (invContextVis S' (visa - {c,ca,cb}))"
-                by (auto simp add: invariant_all_def)
-              hence old_inv1: "inv1 (invContextVis S' (visa - {c, ca, cb}))"
-                and old_inv2: "inv2 (invContextVis S' (visa - {c, ca, cb}))"
-                and old_inv2_h1: "inv2_h1 (invContextVis S' (visa - {c, ca, cb}))"
-                by (auto simp add: inv_def)
-
-
-              show "inv1 (invContextH (callOrigin S'(c \<mapsto> t, ca \<mapsto> t, cb \<mapsto> t)) (transactionOrigin S') (transactionStatus S'(t \<mapsto> Commited))
-                       (insert (c, ca) (insert (ca, cb) (insert (c, cb) (happensBefore S' \<union> vis \<times> {c} \<union> vis \<times> {ca} \<union> vis \<times> {cb}))))
-                       (calls S'(c \<mapsto> Call ''message_chat_read'' [MessageId x4] res, ca \<mapsto> Call ''chat_remove'' [res, MessageId x4] Undef, cb \<mapsto> Call ''message_delete'' [MessageId x4] Undef))
-                       (knownIds S') (invocationOp S') (invocationRes S') (Some visa))"
-              proof (auto simp add: inv1_def)
-                fix cc m
-                assume a0: "crdtSpec_chat_contains_h [cc, m] (mkContext (invContextH (callOrigin S'(c \<mapsto> t, ca \<mapsto> t, cb \<mapsto> t)) (transactionOrigin S') (transactionStatus S'(t \<mapsto> Commited))                           
-                                            (insert (c, ca) (insert (ca, cb) (insert (c, cb) (happensBefore S' \<union> vis \<times> {c} \<union> vis \<times> {ca} \<union> vis \<times> {cb})))) (calls S'(c \<mapsto> Call ''message_chat_read'' [MessageId x4] res, ca \<mapsto> Call ''chat_remove'' [res, MessageId x4] Undef, cb \<mapsto>                            Call ''message_delete'' [MessageId x4] Undef))                           (knownIds S') (invocationOp S') (invocationRes S') (Some visa)))"
-
-                define new_hb where "new_hb \<equiv> (insert (c, ca) (insert (ca, cb) (insert (c, cb) (happensBefore S' \<union> vis \<times> {c} \<union> vis \<times> {ca} \<union> vis \<times> {cb}))))"
-                define new_calls where "new_calls = (calls S'(c \<mapsto> Call ''message_chat_read'' [MessageId x4] res, ca \<mapsto> Call ''chat_remove'' [res, MessageId x4] Undef, cb \<mapsto>                            Call ''message_delete'' [MessageId x4] Undef))"
-
-                from a0 
-                have a0': "crdtSpec_chat_contains_h [cc, m] (mkContext (invContextH (callOrigin S'(c \<mapsto> t, ca \<mapsto> t, cb \<mapsto> t)) (transactionOrigin S') (transactionStatus S'(t \<mapsto> Commited))                           
-                                            new_hb new_calls             (knownIds S') (invocationOp S') (invocationRes S') (Some visa)))"
-                  by (auto simp add: new_hb_def new_calls_def)
-
-                from a0' obtain c_add
-                  where cd1: "isCommittedH (callOrigin S'(c \<mapsto> t, ca \<mapsto> t, cb \<mapsto> t)) (transactionStatus S'(t \<mapsto> Commited)) c_add"
-                    and cd2: "c_add \<in> visa"
-                    and cd3: "new_calls c_add \<triangleq> Call ''chat_add'' [cc, m] Undef"
-                    and cd4: "\<And>cr. isCommittedH (callOrigin S'(c \<mapsto> t, ca \<mapsto> t, cb \<mapsto> t)) (transactionStatus S'(t \<mapsto> Commited)) cr \<and>
-                       cr \<in> visa \<and> new_calls cr \<triangleq> Call ''chat_remove'' [cc, m] Undef \<longrightarrow>
-                       (\<exists>caa. (cr, caa) \<in> new_hb \<and>
-                              isCommittedH (callOrigin S'(c \<mapsto> t, ca \<mapsto> t, cb \<mapsto> t)) (transactionStatus S'(t \<mapsto> Commited)) caa \<and>
-                              caa \<in> visa \<and>
-                              isCommittedH (callOrigin S'(c \<mapsto> t, ca \<mapsto> t, cb \<mapsto> t)) (transactionStatus S'(t \<mapsto> Commited)) caa \<and>
-                              caa \<in> visa \<and> new_calls caa \<triangleq> Call ''chat_add'' [cc, m] Undef)"
-                  by (auto simp add: crdtSpec_chat_contains_h_def mkContext_simps split: if_splits)
-
-                have  [simp]: "c_add \<noteq> ca" 
-                  and [simp]: "c_add \<noteq> c"
-                  and [simp]: "c_add \<noteq> cb"
-                  using cd3 by (auto simp add: new_calls_def split: if_splits)
-
-                have "c_add \<in> commitedCalls S'"
-                  using cd1 by (auto simp add: isCommittedH_def commitedCallsH_def no_calls_in_t split: if_splits)
-
-
-              (*we removed a chat message, so if something exists afterwards it should exist before: *)
-                have "crdtSpec_chat_contains_h [cc, m] (mkContext (invContextVis S' (visa - {c, ca, cb})))"
-                  apply (auto simp add: crdtSpec_chat_contains_h_def mkContext_def) 
-                   apply (rule_tac x=c_add in exI)
-                  using cd3 apply (auto simp add: new_calls_def  invContextH_def restrict_map_def restrict_relation_def cd2 `c_add \<in> commitedCalls S'`)[1]
-                proof -
-                  show " \<exists>caa. (cr, caa) \<in> happensBefore (invContextVis S' (visa - {c, ca, cb})) |r (visa - {c, ca, cb}) \<and>
-                    (calls (invContextVis S' (visa - {c, ca, cb})) |` (visa - {c, ca, cb})) caa \<triangleq> Call ''chat_add'' [cc, m] Undef "
-                    if "(calls (invContextVis S' (visa - {c, ca, cb})) |` (visa - {c, ca, cb})) cr \<triangleq> Call ''chat_remove'' [cc, m] Undef" 
-                    for cr
-                  proof (cases "isCommittedH (callOrigin S'(c \<mapsto> t, ca \<mapsto> t, cb \<mapsto> t)) (transactionStatus S'(t \<mapsto> Commited)) cr \<and>
-                       cr \<in> visa \<and> new_calls cr \<triangleq> Call ''chat_remove'' [cc, m] Undef")
-                    case True
-                    then show ?thesis 
-                      using cd4[where cr=cr] apply auto
-                      apply (rule_tac x=caa in exI)
-                      apply (auto simp add: restrict_map_def restrict_relation_def commitedCallsH_def invContextH_def split: if_splits)[1]
-
-
-                  next
-                    case False
-                    then show ?thesis sorry
-                  qed
-
-                    
-                    apply auto
-                       apply (auto simp add: restrict_map_def restrict_relation_def commitedCallsH_def invContextH_def split: if_splits)[1]
-
-
-                qed
-
-                with old_inv1 
-                have "crdtSpec_message_exists_h [m] (mkContext (invContextVis S' (visa - {c, ca, cb})))"
-                  by (auto simp add: inv1_def)
-
-                from this obtain cc 
-                  where [simp]: "cc \<noteq> c" 
-                    and [simp]: "cc \<noteq> ca"
-                    and [simp]: "cc \<noteq> cb"
-                    and allDeletesOverridden: "\<And>cc. cc \<in> visa \<longrightarrow>
-                calls S' cc \<triangleq> Call ''message_delete'' [m] Undef \<longrightarrow>
-                isCommitted S' cc \<longrightarrow>
-                cc = c \<or> cc = ca \<or> cc = cb \<or> (\<exists>c'. (cc, c') \<in> happensBefore S' |r Collect (isCommitted S') |r (visa - {c, ca, cb})) \<and>
-                                              is_message_updateH m (Call ''message_delete'' [m] Undef)"
-                    and [simp]: "cc \<in> visa"
-                    and "isCommitted S' cc"
-                    and "is_message_update S' cc m"
-                  by (auto simp add: crdtSpec_message_exists_h_def is_message_update_vis_simps mkContext_def invContextH_def  restrict_map_def commitedCallsH_def split: if_splits)
-
-                have "(c, cb) \<notin> happensBefore S'" for c
-                  using c16 c2 wellFormed_happensBefore_calls_r by blast
-
-
-
-
-
-
-                show "crdtSpec_message_exists_h [m]              (mkContext (invContextH (callOrigin S'(c \<mapsto> t, ca \<mapsto> t, cb \<mapsto> t)) (transactionOrigin S') (transactionStatus S'(t \<mapsto> Commited))                           (insert (c, ca) (insert (ca, cb) (insert (c, cb) (happensBefore S' \<union> vis \<times> {c} \<union> vis \<times> {ca} \<union> vis \<times> {cb}))))                           (calls S'(c \<mapsto> Call ''message_chat_read'' [MessageId x4] res, ca \<mapsto> Call ''chat_remove'' [res, MessageId x4] Undef, cb \<mapsto>                            Call ''message_delete'' [MessageId x4] Undef))                           (knownIds S') (invocationOp S') (invocationRes S') (Some visa)))"
-                proof (simp add: crdtSpec_message_exists_h_def, intro conjI exI allI; clarsimp?)
-                  show "is_message_update
-                     (mkContext (invContextH (callOrigin S'(c \<mapsto> t, ca \<mapsto> t, cb \<mapsto> t)) (transactionOrigin S') (transactionStatus S'(t \<mapsto> Commited))
-                                  (insert (c, ca) (insert (ca, cb) (insert (c, cb) (happensBefore S' \<union> vis \<times> {c} \<union> vis \<times> {ca} \<union> vis \<times> {cb}))))
-                                  (calls S'(c \<mapsto> Call ''message_chat_read'' [MessageId x4] res, ca \<mapsto> Call ''chat_remove'' [res, MessageId x4] Undef, cb \<mapsto> Call ''message_delete'' [MessageId x4] Undef))
-                                  (knownIds S') (invocationOp S') (invocationRes S') (Some visa)))
-                     cc m"
-                    using `is_message_update S' cc m`  apply (auto simp add: is_message_update_vis_simps is_message_updateH_simp split: option.splits)
-                    by (smt \<open>isCommitted S' cc\<close> fun_upd_other fun_upd_same isCommittedH_def)
-
-                  show " (\<exists>c'. (cc, c') \<in> happensBefore
-                                               (mkContext (invContextH (callOrigin S'(c \<mapsto> t, ca \<mapsto> t, cb \<mapsto> t)) (transactionOrigin S') (transactionStatus S'(t \<mapsto> Commited))
-                                                            (insert (c, ca) (insert (ca, cb) (insert (c, cb) (happensBefore S' \<union> vis \<times> {c} \<union> vis \<times> {ca} \<union> vis \<times> {cb}))))
-                                                            (calls S'(c \<mapsto> Call ''message_chat_read'' [MessageId x4] res, ca \<mapsto> Call ''chat_remove'' [res, MessageId x4] Undef, cb \<mapsto>
-                                                             Call ''message_delete'' [MessageId x4] Undef))
-                                                            (knownIds S') (invocationOp S') (invocationRes S') (Some visa)))) \<and>
-                            is_message_updateH m (Call ''message_delete'' [m] Undef)" 
-                    if "calls (mkContext (invContextH (callOrigin S'(c \<mapsto> t, ca \<mapsto> t, cb \<mapsto> t)) (transactionOrigin S') (transactionStatus S'(t \<mapsto> Commited))
-                             (insert (c, ca) (insert (ca, cb) (insert (c, cb) (happensBefore S' \<union> vis \<times> {c} \<union> vis \<times> {ca} \<union> vis \<times> {cb}))))
-                             (calls S'(c \<mapsto> Call ''message_chat_read'' [MessageId x4] res, ca \<mapsto> Call ''chat_remove'' [res, MessageId x4] Undef, cb \<mapsto>
-                              Call ''message_delete'' [MessageId x4] Undef))
-                             (knownIds S') (invocationOp S') (invocationRes S') (Some visa)))
-                             cc \<triangleq>  Call ''message_delete'' [m] Undef"
-                    for cc
-                  proof -
-                    from that have ???
-                      apply (auto simp add: mkContext_def invContextH_def commitedCallsH_def split: if_splits)
-
-                    using allDeletesOverridden[where cc=cc]
-                    apply (auto simp add: mkContext_def invContextH_def commitedCallsH_def )
-                              apply (auto split: if_splits)[1]
-
-                    find_theorems invContextH
-
-                sorry
-              show "inv2 (invContextH (callOrigin S'(c \<mapsto> t, ca \<mapsto> t, cb \<mapsto> t)) (transactionOrigin S') (transactionStatus S'(t \<mapsto> Commited))
-                       (insert (c, ca) (insert (ca, cb) (insert (c, cb) (happensBefore S' \<union> vis \<times> {c} \<union> vis \<times> {ca} \<union> vis \<times> {cb}))))
-                       (calls S'(c \<mapsto> Call ''message_chat_read'' [MessageId x4] res, ca \<mapsto> Call ''chat_remove'' [res, MessageId x4] Undef, cb \<mapsto> Call ''message_delete'' [MessageId x4] Undef))
-                       (knownIds S') (invocationOp S') (invocationRes S') (Some visa))"
-                sorry
-              show "inv2_h1 (invContextH (callOrigin S'(c \<mapsto> t, ca \<mapsto> t, cb \<mapsto> t)) (transactionOrigin S') (transactionStatus S'(t \<mapsto> Commited))
-                    (insert (c, ca) (insert (ca, cb) (insert (c, cb) (happensBefore S' \<union> vis \<times> {c} \<union> vis \<times> {ca} \<union> vis \<times> {cb}))))
-                    (calls S'(c \<mapsto> Call ''message_chat_read'' [MessageId x4] res, ca \<mapsto> Call ''chat_remove'' [res, MessageId x4] Undef, cb \<mapsto> Call ''message_delete'' [MessageId x4] Undef))
-                    (knownIds S') (invocationOp S') (invocationRes S') (Some visa))"
-                sorry
-            qed
-
-
-            show "example_chat.inv (invContextH (callOrigin S'(c \<mapsto> t, ca \<mapsto> t, cb \<mapsto> t)) (transactionOrigin S') (transactionStatus S'(t \<mapsto> Commited)) (insert (c, ca) (insert (ca, cb) (insert (c, cb) (happensBefore S' \<union> vis \<times> {c} \<union> vis \<times> {ca} \<union> vis \<times> {cb})))) (calls S'(c \<mapsto> Call ''message_chat_read'' [MessageId x4] res, ca \<mapsto> Call ''chat_remove'' [res, MessageId x4] Undef, cb \<mapsto> Call ''message_delete'' [MessageId x4] Undef)) (knownIds S' \<union> uniqueIds Undef) (invocationOp S') (invocationRes S'(i \<mapsto> Undef)) (Some visa))"
-              if c0: "transactionStatus S t = None"
-                and c1: "invariant_all S'"
-                and c2: "state_wellFormed S'"
-                and c3: "state_monotonicGrowth S S'"
-                and c4: "localState S' i \<triangleq> lsInit\<lparr>ls_id := MessageId x4, ls_pc := Suc 0\<rparr>"
-                and c5: "currentProc S' i \<triangleq> deleteMessageImpl"
-                and c6: "currentTransaction S' i \<triangleq> t"
-                and c7: "transactionOrigin S' t \<triangleq> i"
-                and c8: "\<forall>c. callOrigin S' c \<noteq> Some t"
-                and c9: "calls S' c = None"
-                and c10: "crdtSpec ''message_chat_read'' [MessageId x4] (getContextH (calls S') (happensBefore S') (Some vis)) res"
-                and c11: "visibleCalls S' i \<triangleq> vis"
-                and c12: "ca \<noteq> c"
-                and c13: "calls S' ca = None"
-                and c14: "cb \<noteq> c"
-                and c15: "cb \<noteq> ca"
-                and c16: "calls S' cb = None"
-                and c17: "\<And>ctxt procName args. finite (dom (calls ctxt)) \<Longrightarrow> Ex (crdtSpec procName args ctxt)"
-                and c18: "consistentSnapshot (S'\<lparr>calls := calls S'(c \<mapsto> Call ''message_chat_read'' [MessageId x4] res, ca \<mapsto> Call ''chat_remove'' [res, MessageId x4] Undef, cb \<mapsto> Call ''message_delete'' [MessageId x4] Undef), callOrigin := callOrigin S'(c \<mapsto> t, ca \<mapsto> t, cb \<mapsto> t), happensBefore := insert (c, ca) (insert (ca, cb) (insert (c, cb) (happensBefore S' \<union> vis \<times> {c} \<union> vis \<times> {ca} \<union> vis \<times> {cb}))), currentTransaction := (currentTransaction S')(i := None), transactionStatus := transactionStatus S'(t \<mapsto> Commited), localState := (localState S')(i := None), currentProc := (currentProc S')(i := None), visibleCalls := (visibleCalls S')(i := None), invocationRes := invocationRes S'(i \<mapsto> Undef), knownIds := knownIds S' \<union> uniqueIds Undef\<rparr>) visa"
-              for  t S' c res vis ca cb visa
-            proof -
-              from c18
-              have c18': "consistentSnapshot (S'\<lparr>calls := calls S'(c \<mapsto> Call ''message_chat_read'' [MessageId x4] res, ca \<mapsto> Call ''chat_remove'' [res, MessageId x4] Undef, cb \<mapsto> Call ''message_delete'' [MessageId x4] Undef), callOrigin := callOrigin S'(c \<mapsto> t, ca \<mapsto> t, cb \<mapsto> t), visibleCalls := visibleCalls S'(i \<mapsto> insert cb (insert ca (insert c vis))), happensBefore := insert (c, ca) (insert (ca, cb) (insert (c, cb) (happensBefore S' \<union> vis \<times> {c} \<union> vis \<times> {ca} \<union> vis \<times> {cb}))), localState := localState S'(i \<mapsto> lsInit\<lparr>ls_id := MessageId x4, ls_c := res, ls_pc := 5\<rparr>), currentTransaction := (currentTransaction S')(i := None), transactionStatus := transactionStatus S'(t \<mapsto> Commited)\<rparr>) visa"
-                by (auto simp add: consistentSnapshot_def)
-
-              from h[OF c0 c1 c2 c3 c4 c5 c6 c7 c8 c9 c10 c11 c12 c13 c14 c15 c16 c17 c18']
-              show "?thesis"
-                by (meson example_chat.inv_def inv1_unchanged inv2_h1_unchanged inv2_unchanged)
-            qed
-          qed
-        qed
-
-
-        text {* send message *}
-        show "checkCorrectAll progr S i"
-          if c0: "invocationOp S i \<triangleq> (''sendMessage'', [UserId x2, String x1, ChatId x3])"
-            and c1: "currentProc S i \<triangleq> sendMessageImpl"
-            and c2: "localState S i \<triangleq> lsInit\<lparr>ls_from := UserId x2, ls_content := String x1, ls_to := ChatId x3\<rparr>"
-            and c3: "uniqueIdsInList [UserId x2, String x1, ChatId x3] \<subseteq> knownIds S"
-          for  x2 x1 x3
-          sorry
-
-
-
-      qed
 
 end
